Blanc.lean
@@ -1,1 +1,17 @@
-import «Blanc».Deployer
+import «Blanc».Weth
+
+partial def Bytes.chunks (bs : Bytes) : List Bytes :=
+  match bs.splitAt 32 with
+  | (_, []) => [bs]
+  | (bs', bs'') => bs' :: chunks bs''
+
+def Bytes.toHexString (bs : Bytes) : String :=
+  "hex\"" ++ List.foldr (λ b s => b.toString ++ s) "\"" bs
+
+def WethByteCode : String :=
+  List.foldr
+     (λ s0 s1 => s0 ++ "\n" ++ s1)
+     "" <| List.map Bytes.toHexString (Option.getD weth.compile []).chunks
+
+def main : IO Unit :=
+  IO.println WethByteCode
